execution/tests/FA2Tests/FA2Gens.v
@@ -1,0 +1,214 @@
+From ConCert Require Import Blockchain LocalBlockchain FA2Token FA2Interface.
+From ConCert Require Import Serializable.
+From ConCert Require Import LocalBlockchainTests.
+(* From Coq Require Import Morphisms. *)
+From ConCert Require Import Extras.
+From ConCert Require Import Containers.
+From ConCert Require Import BoundedN.
+Global Set Warnings "-extraction-logical-axiom".
+
+From QuickChick Require Import QuickChick. Import QcNotation.
+From ExtLib.Structures Require Import Functor Applicative.
+From ConCert.Execution.QCTests Require Import 
+	ChainGens TestUtils ChainPrinters SerializablePrinters TraceGens FA2Printers TestContracts.
+From RecordUpdate Require Import RecordUpdate.
+From Coq Require Import ZArith List.
+Import ListNotations.
+Import RecordSetNotations.
+(* For monad notations *)
+From ExtLib.Structures Require Import Monads.
+Import MonadNotation. Open Scope monad_scope.
+(* Notation "f 'o' g" := (compose f g) (at level 50). *)
+
+Module Type FA2TestsInfo.
+  Parameter fa2_contract_addr : Address.
+  Parameter fa2_client_addr : Address.
+  Parameter fa2_hook_addr : Address.
+End FA2TestsInfo.
+
+Module FA2Gens (Info : FA2TestsInfo).
+Import Info.
+Arguments SerializedValue : clear implicits.
+Arguments deserialize : clear implicits.
+Arguments serialize : clear implicits.
+Definition LocalChainBase : ChainBase := ChainGens.LocalChainBase.
+
+(* --------------------- FA2 Contract Generators --------------------- *)
+Section FA2ContractGens.
+
+(* 
+  generates a fa2 transfer message, where the following properties hold:
+  - 0 < amount <= to_ balance 
+  - if operators are allowed, then caller must be a valid operator for this transfer
+  - token_id is among existing token_ids of the FA2 Token state.
+*)
+(* Definition gTransfer : G transfer := 
+  from <- arbitrary ;;
+  to <- arbitrary ;;
+  tokenid <- arbitrary ;;
+  amount <- arbitrary ;;
+  returnGen {|
+    from_ := from;
+    to_ := to;
+    transfer_token_id := tokenid;
+    amount := amount;
+  |}.
+
+Local Open Scope N_scope.
+Definition valid_transfer_prop state trx :=
+  let from_balance := address_balance trx.(transfer_token_id) trx.(from_) state in
+  (trx.(amount) <=? from_balance ) && (
+    isSome (FMap.find trx.(transfer_token_id) state.(tokens))
+  ).
+Definition gValidTransfer (state : FA2Token.State) :=
+  suchThatMaybe gTransfer (valid_transfer_prop state). *)
+
+Definition policy_allows_operator_transfer (policy : permissions_descriptor) : bool := 
+  match policy.(descr_operator) with
+  | operator_transfer_permitted => true 
+  | operator_transfer_denied => false
+  end.
+
+Definition policy_allows_self_transfer (policy : permissions_descriptor) : bool := 
+  match policy.(descr_self) with
+  | self_transfer_permitted => true 
+  | self_transfer_denied => false
+  end .
+
+(* TODO: check specification if transfers between contract addresses are allowed *)
+Definition gTransferFrom (lc : LocalChain) 
+                         (state : FA2Token.State) 
+                         (ledger : TokenLedger)
+                         (caller : Address) 
+                         : G (option Address) :=
+  let policy := state.(permission_policy) in
+  if policy_disallows_operator_transfer policy then
+    if policy_allows_self_transfer policy then
+      (* caller and from must be the same *)
+      returnGen (Some caller)
+    else
+      returnGen None
+  else
+    (* allows operator transfer, but not self transfer, so caller != from *)
+    from <- (gAddrFromLCWithoutAddrs lc [caller]) ;;
+    returnGen (Some from)
+.
+
+Local Open Scope N_scope.
+Definition gSingleTransfer (lc : LocalChain)
+                           (state : FA2Token.State)
+                           (caller : Address)
+                           : G (option transfer) :=
+  p <- (sampleFMapOpt state.(tokens)) ;;
+  let tokenid := fst p in
+  match FMap.find tokenid state.(assets) with
+  | Some ledger =>
+    from <- (gTransferFrom lc state ledger caller) ;;
+    bindGenOpt (gAddrFromLCWithoutAddrs lc [from])
+    (fun to =>
+      let from_balance := with_default 0 (FMap.find from ledger.(balances)) in
+      if from_balance =? 0 then
+        returnGen None
+      else
+        amount <- choose (0, from_balance) ;;
+        returnGen (
+          Some {|
+            from_ := from;
+            to_ := to;
+            transfer_token_id := tokenid;
+            amount := amount;
+          |})
+    )
+  | None => returnGen None
+  end.
+
+
+Fixpoint gTransfersFix (lc : LocalChain)
+                     (state : FA2Token.State)
+                     (caller : Address)
+                     (maxNrTransfers : nat)
+                     (acc : list transfer)
+                     : G (option (list transfer)) :=
+  match maxNrTransfers with
+  | 0%nat => match acc with
+             | [] => returnGen None
+             | _ => returnGen (Some acc) 
+             end
+  | S n => trx <-  (gSingleTransfer lc state caller) ;;
+           gTransfersFix lc state caller n (trx :: acc)
+  end.
+
+Definition gTransfer (lc : LocalChain)
+                     (state : FA2Token.State)
+                     (caller : Address)
+                     (maxNrTransfers : nat)
+                     : G (option FA2Token.Msg) := 
+  trxs <- (gTransfersFix lc state caller maxNrTransfers []) ;;
+  returnGen (Some (msg_transfer trxs)).
+  
+
+Local Close Scope N_scope.
+Definition gFA2TokenAction (lc : LocalChain) : G (option Action) :=
+  let mk_call caller_addr msg :=
+		returnGen (Some {|
+			act_from := caller_addr;
+			act_body := act_call fa2_contract_addr 0%Z (serialize FA2Token.Msg _ msg) 
+    |}) in
+  match FMap.find fa2_contract_addr (lc_contract_state_deserialized FA2Token.State lc) with
+  | Some fa2_state => 
+    backtrack [
+      (1, caller <- gAddrFromLCWithoutAddrs lc [] ;;
+          trx <- gTransfer lc fa2_state caller 1 ;; 
+          mk_call caller trx
+      )
+    ]
+  | None => returnGen None
+  end.
+
+End FA2ContractGens.
+
+
+(* --------------------- FA2 Client Generators --------------------- *)
+Section FA2ClientGens.
+Let client_other_msg := @other_msg _ FA2ClientMsg _.
+
+Definition gClientMsg : G ClientMsg := 
+  let params := Build_is_operator_param 
+    (Build_operator_param zero_address zero_address all_tokens)
+    (Build_callback is_operator_response None) in
+  returnGen (client_other_msg (Call_fa2_is_operator params)).
+
+Definition gClientAction := 
+  msg <- gClientMsg ;;
+  returnGen (Some (
+    build_act person_1 (
+      act_call fa2_contract_addr 0%Z (serialize ClientMsg _ msg)
+    )
+  )).
+
+End FA2ClientGens.
+
+(* Definition gFA2ChainTraceList max_acts_per_block lc length := 
+  gLocalChainTraceList_fix lc (fun _ _=> 
+    gClientAction) length max_acts_per_block.
+
+Definition token_reachableFrom (lc : LocalChain) pf : Checker := 
+  @reachableFrom AddrSize lc (gFA2ChainTraceList 1) pf.
+
+Definition token_reachableFrom_implies_reachable (lc : LocalChain) pf1 pf2 : Checker := 
+  reachableFrom_implies_reachable lc (gFA2ChainTraceList 1) pf1 pf2. *)
+
+(* --------------------- FA2 Hook Generators --------------------- *)
+Section FA2HookGens.
+  
+
+End FA2HookGens.
+End FA2Gens.
+
+Module DummyTestInfo <: FA2TestsInfo.
+  Definition fa2_contract_addr := zero_address.
+  Definition fa2_client_addr := zero_address.
+  Definition fa2_hook_addr := zero_address.
+End DummyTestInfo.
+Module MG := FA2Gens.FA2Gens DummyTestInfo. Import MG.
+(* Sample gClientMsg. *)
